thy/IP_Addresses/IPAddr.thy
@@ -2,14 +2,13 @@
     Authors:    Cornelius Diekmann
 *)
 theory IPAddr
-imports Main
-  NumberWang
-  Hs_Compat
-  WordInterval
+imports NumberWang
+        Hs_Compat
+        WordInterval
 begin
 
 section \<open>Modelling IP Adresses\<close>
-  text\<open>An IP address is basically a unsigned integer.
+  text\<open>An IP address is basically an unsigned integer.
     We model IP addresses of arbitrary lengths.
 
     We will write @{typ "'i::len word"} for IP addresses of length @{term "len_of TYPE('i::len)"}.
@@ -19,7 +18,7 @@ section \<open>Modelling IP Adresses\<close>
 
     The files @{file "IPv4Addr.thy"} @{file "IPv6Addr.thy"} concrete this for IPv4 and IPv6.\<close>
 
-  text\<open>The maximum IP addres\<close>
+  text\<open>The maximum IP address\<close>
   definition max_ip_addr :: "'i::len word" where 
     "max_ip_addr \<equiv> of_nat ((2^(len_of(TYPE('i)))) - 1)"
 
@@ -31,7 +30,7 @@ section \<open>Modelling IP Adresses\<close>
   lemma range_0_max_UNIV: "UNIV = {0 .. max_ip_addr}" (*not in the simp set, for a reason*)
     by(simp add: max_ip_addr_max_word) fastforce
 
-  lemma size_ipaddr: "size (x::'i::len word) = len_of(TYPE('i))" by(simp add:word_size)
+  lemma "size (x::'i::len word) = len_of(TYPE('i))" by(simp add:word_size)
 
 subsection\<open>Sets of IP addresses\<close>
   (*Warning, not executable!*)
@@ -44,7 +43,8 @@ subsection\<open>Sets of IP addresses\<close>
         {network_prefix .. network_prefix OR (NOT netmask)}"
   
   text\<open>Example (pseudo syntax):
-    @{const ipset_from_netmask}@{text "192.168.1.129  255.255.255.0 = {192.168.1.0 .. 192.168.1.255}"}\<close>
+    @{const ipset_from_netmask}@{text "192.168.1.129  255.255.255.0"} =
+        @{text "{192.168.1.0 .. 192.168.1.255}"}\<close>
 
   text{*A network mask of all ones (i.e. @{term "(- 1)::'i::len word"}).*}
   lemma ipset_from_netmask_minusone: 
@@ -56,28 +56,29 @@ subsection\<open>Sets of IP addresses\<close>
     "ipset_from_netmask ip 0 = UNIV" by (auto simp add: ipset_from_netmask_def) 
 
 
-  text\<open>Specifying sets in CIDR notation: 192.168.0.0/24\<close>
+  text\<open>Specifying sets in Classless Inter-domain Routing (CIDR )notation: 192.168.0.0/24\<close>
   definition ipset_from_cidr ::"'i::len word \<Rightarrow> nat \<Rightarrow> 'i::len word set" where
-    "ipset_from_cidr addr pflength \<equiv> ipset_from_netmask addr ((mask pflength) << (len_of(TYPE('i)) - pflength))"
+    "ipset_from_cidr addr pflength \<equiv>
+       ipset_from_netmask addr ((mask pflength) << (len_of(TYPE('i)) - pflength))"
 
   text\<open>Example (pseudo syntax):
-    @{const ipset_from_cidr}@{text "192.168.1.129 24  = {192.168.1.0 .. 192.168.1.255}"}\<close>
+    @{const ipset_from_cidr}@{text "192.168.1.129 24"} = @{text "{192.168.1.0 .. 192.168.1.255}"}\<close>
 
-  (*TODO: does this help?*)
+  (*does this simplify stuff?*)
   lemma "(case ipcidr of (base, len) \<Rightarrow> ipset_from_cidr base len) = uncurry ipset_from_cidr ipcidr"
     by(simp add: uncurry_case_stmt)
 
   lemma ipset_from_cidr_0: "ipset_from_cidr ip 0 = UNIV"
     by(auto simp add: ipset_from_cidr_def ipset_from_netmask_def Let_def)
 
-  text\<open>A prefix lengths of word size gives back the singleton set with the IP address.
+  text\<open>A prefix length of word size gives back the singleton set with the IP address.
        Example: @{text "192.168.1.2/32 = {192.168.1.2}"}\<close>
   lemma ipset_from_cidr_wordlength: 
-    fixes foo :: "'i::len word"
-    shows "ipset_from_cidr foo (len_of TYPE('i)) = {foo}"
+    fixes ip :: "'i::len word"
+    shows "ipset_from_cidr ip (len_of TYPE('i)) = {ip}"
     by(simp add: ipset_from_cidr_def ipset_from_netmask_def Let_def mask_def)
 
-  text\<open>Alternative definition: considering words as bit lists:\<close>
+  text\<open>Alternative definition: Considering words as bit lists:\<close>
   lemma ipset_from_cidr_bl:
     fixes addr :: "'i::len word"
     shows "ipset_from_cidr addr pflength \<equiv> 
@@ -88,7 +89,9 @@ subsection\<open>Sets of IP addresses\<close>
   lemma ipset_from_cidr_alt: 
     fixes pre :: "'i::len word"
     shows "ipset_from_cidr pre len =
-            {(pre AND ((mask len) << (len_of(TYPE('i)) - len))) .. pre OR (mask (len_of(TYPE('i)) - len))}"
+            {pre AND (mask len << len_of TYPE('i) - len)
+             ..
+             pre OR mask (len_of TYPE('i) - len)}"
     apply(simp add: ipset_from_cidr_def ipset_from_netmask_def Let_def)
     apply(simp add: Word.word_oa_dist)
     apply(simp add: NOT_mask_shifted_lenword)
@@ -97,7 +100,7 @@ subsection\<open>Sets of IP addresses\<close>
   lemma ipset_from_cidr_alt2:
     fixes base ::"'i::len word"
     shows "ipset_from_cidr base len = 
-           ipset_from_netmask base (NOT mask (len_of (TYPE('i)) - len))"
+           ipset_from_netmask base (NOT mask (len_of TYPE('i) - len))"
     apply(simp add: ipset_from_cidr_def)
     using NOT_mask_shifted_lenword by(metis word_not_not)
   
@@ -108,18 +111,17 @@ subsection\<open>Sets of IP addresses\<close>
   text{*Though we can write 192.168.1.2/24, we say that 192.168.0.0/24 is well-formed.*}
   lemma ipset_from_cidr_base_wellforemd: fixes base:: "'i::len word"
     assumes "mask (len_of TYPE('i) - l) AND base = 0"
-      shows "ipset_from_cidr base l = {base .. base || mask (len_of TYPE('i) - l)}"
+      shows "ipset_from_cidr base l = {base .. base OR mask (len_of TYPE('i) - l)}"
   proof -
     have maskshift_eq_not_mask_generic:
       "((mask l << len_of TYPE('i) - l) :: 'i::len word) = NOT mask (len_of TYPE('i) - l)"
       using NOT_mask_shifted_lenword by (metis word_not_not) 
-    
-    have *: "base AND NOT  mask (len_of TYPE('i) - l) = base"
+    have *: "base AND NOT mask (len_of TYPE('i) - l) = base"
       unfolding mask_eq_0_eq_x[symmetric] using assms word_bw_comms(1)[of base] by simp
-    hence **: "base AND NOT mask (len_of TYPE('i) - l) OR mask (len_of TYPE('i) - l) = base OR mask (len_of TYPE('i) - l)"
-      by simp
-  
-    have "ipset_from_netmask base (NOT mask (len_of TYPE('i) - l)) = {base .. base || mask (len_of TYPE('i) - l)}"
+    hence **: "base AND NOT mask (len_of TYPE('i) - l) OR mask (len_of TYPE('i) - l) =
+                base OR mask (len_of TYPE('i) - l)" by simp
+    have "ipset_from_netmask base (NOT mask (len_of TYPE('i) - l)) =
+            {base .. base || mask (len_of TYPE('i) - l)}"
       by(simp add: ipset_from_netmask_def Let_def ** *)
     thus ?thesis by(simp add: ipset_from_cidr_def maskshift_eq_not_mask_generic)
   qed
@@ -139,16 +141,18 @@ subsection\<open>Sets of IP addresses\<close>
 
   lemma ipset_from_netmask_base_mask_consume:
     fixes base :: "'i::len word"
-    shows "ipset_from_netmask (base AND NOT mask (len_of TYPE('i) - m)) (NOT mask (len_of TYPE('i) - m)) =
-            ipset_from_netmask base (NOT mask (len_of TYPE('i) - m))"
+    shows "ipset_from_netmask (base AND NOT mask (len_of TYPE('i) - m))
+                              (NOT mask (len_of TYPE('i) - m))
+            =
+             ipset_from_netmask base (NOT mask (len_of TYPE('i) - m))"
     unfolding ipset_from_netmask_def by(simp)
 
 
   text\<open>Another definition of CIDR notation:
-       All IP addresse which are equal on the first @{text "len - n"} bits\<close>
+       All IP address which are equal on the first @{term "len - n"} bits\<close>
   definition ip_cidr_set :: "'i::len word \<Rightarrow> nat \<Rightarrow> 'i word set" where
-    "ip_cidr_set i r = {j . i AND NOT mask (len_of TYPE('i) - r) = j AND NOT mask (len_of TYPE('i) - r)}"
-
+    "ip_cidr_set i r \<equiv>
+      {j . i AND NOT mask (len_of TYPE('i) - r) = j AND NOT mask (len_of TYPE('i) - r)}"
 
   text\<open>The definitions are equal\<close>
   lemma ipset_from_cidr_eq_ip_cidr_set:
@@ -158,11 +162,9 @@ subsection\<open>Sets of IP addresses\<close>
     have maskshift_eq_not_mask_generic:
       "((mask len << len_of TYPE('a) - len) :: 'a::len word) = NOT mask (len_of TYPE('a) - len)"
       using NOT_mask_shifted_lenword by (metis word_not_not) 
-  
     have 1: "mask (len - m) AND base AND NOT mask (len - m) = 0"
       for len m and base::"'i::len word"
       by(simp add: word_bw_lcs)
-  
     have 2: "mask (len_of TYPE('i) - len) AND pfxm_p = 0 \<Longrightarrow>
            (a \<in> ipset_from_netmask pfxm_p (NOT mask (len_of TYPE('i) - len))) \<longleftrightarrow>
            (pfxm_p = NOT mask (len_of TYPE('i) - len) AND a)" for a::"'i::len word" and pfxm_p
@@ -173,7 +175,6 @@ subsection\<open>Sets of IP addresses\<close>
      apply(simp; fail)
     apply(simp)
     done
-  
     from 2[OF 1, of _ base] have
       "(x \<in> ipset_from_netmask base (~~ mask (len_of TYPE('i) - len))) \<longleftrightarrow>
        (base && ~~ mask (len_of TYPE('i) - len) = x && ~~ mask (len_of TYPE('i) - len))" for x
@@ -200,11 +201,12 @@ subsection\<open>IP Addresses as WordIntervals\<close>
   declare iprange_interval.simps[simp del]
 
   lemma iprange_interval_uncurry: "iprange_interval ipcidr = uncurry WordInterval ipcidr"
-    apply(cases ipcidr)
-    by(simp add: iprange_interval.simps)
+    by(cases ipcidr) (simp add: iprange_interval.simps)
 
-  lemma "wordinterval_to_set (iprange_single ip) = {ip}" by(simp add: iprange_single_def)
-  lemma "wordinterval_to_set (iprange_interval (ip1, ip2)) = {ip1 .. ip2}" by(simp add: iprange_interval.simps)
+  lemma "wordinterval_to_set (iprange_single ip) = {ip}"
+    by(simp add: iprange_single_def)
+  lemma "wordinterval_to_set (iprange_interval (ip1, ip2)) = {ip1 .. ip2}"
+    by(simp add: iprange_interval.simps)
   
   text\<open>Now we can use the set operations on @{typ "'i::len wordinterval"}s\<close>
   term wordinterval_to_set
@@ -235,7 +237,7 @@ subsection\<open>IP Addresses in CIDR Notation\<close>
           network_prefix = (pre AND netmask)
       in network_prefix OR (NOT netmask))"
   definition ipcidr_to_interval :: "('i::len word \<times> nat) \<Rightarrow> ('i word \<times> 'i word)" where
-    "ipcidr_to_interval cidr = (ipcidr_to_interval_start cidr, ipcidr_to_interval_end cidr)"
+    "ipcidr_to_interval cidr \<equiv> (ipcidr_to_interval_start cidr, ipcidr_to_interval_end cidr)"
 
 
   lemma ipset_from_cidr_ipcidr_to_interval:
@@ -248,19 +250,18 @@ subsection\<open>IP Addresses in CIDR Notation\<close>
     "ipcidr_to_interval (base, len) = (s,e) \<Longrightarrow> ipset_from_cidr base len = {s .. e}"
     by (simp add: ipcidr_to_interval_def ipset_from_cidr_ipcidr_to_interval)
 
-
   definition ipcidr_tuple_to_wordinterval :: "('i::len word \<times> nat) \<Rightarrow> 'i wordinterval" where
-    "ipcidr_tuple_to_wordinterval iprng = iprange_interval (ipcidr_to_interval iprng)"
+    "ipcidr_tuple_to_wordinterval iprng \<equiv> iprange_interval (ipcidr_to_interval iprng)"
 
   lemma wordinterval_to_set_ipcidr_tuple_to_wordinterval:
     "wordinterval_to_set (ipcidr_tuple_to_wordinterval (b, m)) = ipset_from_cidr b m"
-    unfolding ipcidr_tuple_to_wordinterval_def ipset_from_cidr_ipcidr_to_interval ipcidr_to_interval_def
+    unfolding ipcidr_tuple_to_wordinterval_def ipset_from_cidr_ipcidr_to_interval
+              ipcidr_to_interval_def
     by(simp add: iprange_interval.simps)
 
   lemma wordinterval_to_set_ipcidr_tuple_to_wordinterval_uncurry:
     "wordinterval_to_set (ipcidr_tuple_to_wordinterval ipcidr) = uncurry ipset_from_cidr ipcidr"
     by(cases ipcidr, simp add: wordinterval_to_set_ipcidr_tuple_to_wordinterval)
-
 
   definition ipcidr_union_set :: "('i::len word \<times> nat) set \<Rightarrow> ('i word) set" where
     "ipcidr_union_set ips \<equiv> \<Union>(base, len) \<in> ips. ipset_from_cidr base len"
@@ -326,16 +327,15 @@ subsection\<open>Clever Operations on IP Addresses in CIDR Notation\<close>
        \<not> ip_cidr_set i2 r2 \<subseteq> ip_cidr_set i1 r1 \<Longrightarrow>
        ip_cidr_set i1 r1 \<inter> ip_cidr_set i2 r2 = {}"
       apply(cases "r1 \<le> r2")
-       using ip_cidr_set_intersect_subset_helper apply blast
+       subgoal using ip_cidr_set_intersect_subset_helper by blast
       apply(cases "r2 \<le> r1")
-       using ip_cidr_set_intersect_subset_helper apply blast
-      apply(simp)
-      done
+       subgoal using ip_cidr_set_intersect_subset_helper by blast
+      by(simp)
   end
 
 
-  lemma ip_cidr_intersect: "
-      \<not> ipset_from_cidr b2 m2 \<subseteq> ipset_from_cidr b1 m1 \<Longrightarrow>
+  lemma ip_cidr_intersect:
+     "\<not> ipset_from_cidr b2 m2 \<subseteq> ipset_from_cidr b1 m1 \<Longrightarrow>
       \<not> ipset_from_cidr b1 m1 \<subseteq> ipset_from_cidr b2 m2 \<Longrightarrow>
       ipset_from_cidr b1 m1 \<inter> ipset_from_cidr b2 m2 = {}"
     apply(simp add: ipset_from_cidr_eq_ip_cidr_set)
@@ -343,26 +343,28 @@ subsection\<open>Clever Operations on IP Addresses in CIDR Notation\<close>
 
   text\<open>Computing the intersection of two IP address ranges in CIDR notation\<close>
   fun ipcidr_conjunct :: "('i::len word \<times> nat) \<Rightarrow> ('i word \<times> nat) \<Rightarrow> ('i word \<times> nat) option" where 
-    "ipcidr_conjunct (base1, m1) (base2, m2) = (if ipset_from_cidr base1 m1 \<inter> ipset_from_cidr base2 m2 = {}
+    "ipcidr_conjunct (base1, m1) (base2, m2) = (
+       if
+         ipset_from_cidr base1 m1 \<inter> ipset_from_cidr base2 m2 = {}
        then
-        None
+         None
        else if 
-        ipset_from_cidr base1 m1 \<subseteq> ipset_from_cidr base2 m2
+         ipset_from_cidr base1 m1 \<subseteq> ipset_from_cidr base2 m2
        then 
-        Some (base1, m1)
+         Some (base1, m1)
        else
-        Some (base2, m2)
+         Some (base2, m2)
       )"
   
-  text{*Intersecting with an address with prefix length zero always yields non-empty result.*}
+  text{*Intersecting with an address with prefix length zero always yields a non-empty result.*}
   lemma ipcidr_conjunct_any: "ipcidr_conjunct a (x,0) \<noteq> None" "ipcidr_conjunct (y,0) b \<noteq> None"
      apply(cases a, simp add: ipset_from_cidr_0 ipset_from_cidr_not_empty)
     by(cases b, simp add: ipset_from_cidr_0 ipset_from_cidr_not_empty)
   
   lemma ipcidr_conjunct_correct: "(case ipcidr_conjunct (b1, m1) (b2, m2)
                                           of Some (bx, mx) \<Rightarrow> ipset_from_cidr bx mx
-                                          |  None \<Rightarrow> {})
-      = (ipset_from_cidr b1 m1) \<inter> (ipset_from_cidr b2 m2)"
+                                          |  None \<Rightarrow> {}) =
+                                   (ipset_from_cidr b1 m1) \<inter> (ipset_from_cidr b2 m2)"
     apply(simp split: split_if_asm)
     using ip_cidr_intersect by fast
   declare ipcidr_conjunct.simps[simp del]
@@ -371,31 +373,38 @@ subsection\<open>Clever Operations on IP Addresses in CIDR Notation\<close>
 subsection\<open>Code Equations\<close>
   text\<open>Executable definition using word intervals\<close>
   lemma ipcidr_conjunct_word[code_unfold]: 
-  "ipcidr_conjunct ips1 ips2 = (if wordinterval_empty (wordinterval_intersection (ipcidr_tuple_to_wordinterval ips1) (ipcidr_tuple_to_wordinterval ips2))
-       then
-        None
-       else if 
-        wordinterval_subset (ipcidr_tuple_to_wordinterval ips1) (ipcidr_tuple_to_wordinterval ips2)
-       then 
-        Some ips1
-       else
-        Some ips2
-      )"
+  "ipcidr_conjunct ips1 ips2 = (
+     if
+      wordinterval_empty (wordinterval_intersection
+                            (ipcidr_tuple_to_wordinterval ips1) (ipcidr_tuple_to_wordinterval ips2))
+     then
+       None
+     else if 
+       wordinterval_subset (ipcidr_tuple_to_wordinterval ips1) (ipcidr_tuple_to_wordinterval ips2)
+     then 
+       Some ips1
+     else
+       Some ips2
+     )"
   apply(simp)
   apply(cases ips1, cases ips2, rename_tac b1 m1 b2 m2, simp)
-  apply(auto simp add: wordinterval_to_set_ipcidr_tuple_to_wordinterval ipcidr_conjunct.simps split:split_if_asm)
+  apply(auto simp add: wordinterval_to_set_ipcidr_tuple_to_wordinterval ipcidr_conjunct.simps
+             split: split_if_asm)
   done
 
   (*with the code_unfold lemma before, this works!*)
   lemma "ipcidr_conjunct (0::32 word,0) (8,1) = Some (8, 1)" by eval
-
+  export_code ipcidr_conjunct checking SML
 
   text\<open>making element check executable\<close>
   lemma addr_in_ipset_from_netmask_code[code_unfold]: 
-    "addr \<in> (ipset_from_netmask base netmask) \<longleftrightarrow> (base AND netmask) \<le> addr \<and> addr \<le> (base AND netmask) OR (NOT netmask)"
+    "addr \<in> (ipset_from_netmask base netmask) \<longleftrightarrow>
+      (base AND netmask) \<le> addr \<and> addr \<le> (base AND netmask) OR (NOT netmask)"
     by(simp add: ipset_from_netmask_def Let_def)
-  lemma addr_in_ipset_from_cidr_code[code_unfold]: "(addr::'i::len word) \<in> (ipset_from_cidr pre len) \<longleftrightarrow> 
-              (pre AND ((mask len) << (len_of (TYPE('i)) - len))) \<le> addr \<and> addr \<le> pre OR (mask (len_of (TYPE('i)) - len))"
+  lemma addr_in_ipset_from_cidr_code[code_unfold]:
+    "(addr::'i::len word) \<in> (ipset_from_cidr pre len) \<longleftrightarrow> 
+       (pre AND ((mask len) << (len_of TYPE('i) - len))) \<le> addr \<and>
+        addr \<le> pre OR (mask (len_of TYPE('i) - len))"
   unfolding ipset_from_cidr_alt by simp
 
 
